theories/examples/template_adequacy_ocpl.v
@@ -153,7 +153,7 @@ Theorem ocpl_template_adequacy `{MachineParameters} (Σ : gFunctors)
     (m m': Mem) (reg reg': Reg) (es: list cap_lang.expr):
   is_initial_memory P Adv (library layout) P_tbl Adv_tbl m →
   is_initial_registers P Adv (library layout) P_tbl Adv_tbl reg r_adv →
-  Forall (λ w, is_z w = true) (prog_instrs Adv) →
+  Forall (adv_condition Adv) (prog_instrs Adv) →
 
   let filtered_map := λ (m : gmap Addr Word), filter (fun '(a, _) => a ∉ minv_dom (flag_inv layout)) m in
   (∀ `{memG Σ', regG Σ', sealStoreG Σ', logrel_na_invs Σ', subG Σ Σ'} rmap,
